Annotate AES/GCM specs to indicate endianness, fix endianness issues

src/arch/Types_s.fst
@@ -4,6 +4,7 @@ open Words_s
 open Words.Two_s
 open Words.Four_s
 open Words.Seq_s
+open FStar.Seq
 open Collections.Seqs_s
 
 unfold let nat8 = Words_s.nat8
@@ -36,31 +37,38 @@ let quad32_xor (x y:quad32) : quad32 = four_map2 nat32_xor x y
 
 let select_word (q:quad32) (selector:twobits) : nat32 = four_select q selector
 let insert_nat32 (q:quad32) (n:nat32) (i:twobits) : quad32 = four_insert q n i
-let insert_nat64 (q:quad32) (n:nat64) (high:bool) : quad32 = 
-  let Mktwo lo hi = nat_to_two 32 n in
-  if high then
-    let q' = four_insert q lo 2 in
-    let q' = four_insert q' hi 3 in
-    q'
-  else
-    let q' = four_insert q lo 0 in
-    let q' = four_insert q' hi 1 in
-    q'
+let insert_nat64 (q:quad32) (n:nat64) (i:nat1) : quad32 =
+  two_two_to_four (two_insert (four_to_two_two q) (nat_to_two 32 n) i)
     
 open FStar.Seq
 
-let be_bytes_to_nat32 (b:seq4 nat8) : Tot nat32 =
+let be_bytes_to_nat32 (b:seq4 nat8) : nat32 =
   four_to_nat 8 (seq_to_four_BE b)
 
-let nat32_to_be_bytes (n:nat32) : Tot (b:seq4 nat8 { be_bytes_to_nat32 b == n }) =
+let nat32_to_be_bytes (n:nat32) : b:seq4 nat8 { be_bytes_to_nat32 b == n } =
   let b = four_to_seq_BE (nat_to_four 8 n) in
   assume (be_bytes_to_nat32 b == n);
   b
 
-assume val be_bytes_to_nat32_to_be_bytes (b:seq nat8 {length b == 4}) : 
+assume val be_bytes_to_nat32_to_be_bytes (b:seq4 nat8) :
   Lemma (nat32_to_be_bytes (be_bytes_to_nat32 b) == b)
 
-let reverse_bytes_nat32 (n:nat32) : Tot (nat32) =
+let le_bytes_to_quad32 (b:seqn 16 nat8) : quad32 =
+  seq_to_four_LE (seq_map (four_to_nat 8) (seq_to_seq_four_LE b))
+
+let be_bytes_to_quad32 (b:seqn 16 nat8) : quad32 =
+  seq_to_four_BE (seq_map (four_to_nat 8) (seq_to_seq_four_BE b))
+
+let le_quad32_to_bytes (b:quad32) : seqn 16 nat8 =
+  seq_four_to_seq_LE (seq_map (nat_to_four 8) (four_to_seq_LE b))
+
+let le_seq_quad32_to_bytes (b:seq quad32) : seq nat8 =
+  seq_nat32_to_seq_nat8_LE (seq_four_to_seq_LE b)
+
+let le_bytes_to_seq_quad32 (b:seq nat8{length b % 16 == 0}) : seq quad32 =
+  seq_to_seq_four_LE (seq_nat8_to_seq_nat32_LE b)
+
+let reverse_bytes_nat32 (n:nat32) : nat32 =
   be_bytes_to_nat32 (reverse_seq (nat32_to_be_bytes n))
 
 assume val reverse_bytes_quad32 (q:quad32) : quad32
