src/crypto/aes/GF128_s.fsti
@@ -16,7 +16,3 @@ let gf128_mul (a b:poly) : poly = mod (mul a b) gf128_modulus
 
 let gf128_to_quad32 (a:poly) : quad32 = to_quad32 (reverse a 127)
 let gf128_of_quad32 (q:quad32) : poly = reverse (of_quad32 q) 127
-
-// TODO: get rid of these, they aren't used in GCM:
-let to_quad32 = Math.Poly2.Bits_s.to_quad32
-let of_quad32 = Math.Poly2.Bits_s.of_quad32
